Update AcceptorTheory.v

AcceptorTheory.v
@@ -1,7 +1,50 @@
 Require Import StateMachines.Preliminaries.
 Require Import StateMachines.Concepts.
+Require Import StateMachines.MachineTheory.
 Import ListNotations.
 Import MACHINE.
+Import ACCEPTOR.
 
 Section AcceptorTheory.
+Variables (m : Machine) (a : @Acceptor m).
+
+Definition acc0 (f : state m → list (input m) → Prop)
+:= ∀ s : state m, f s [] ↔ acceptant a s.
+Definition accT (f : state m → list (input m) → Prop)
+:= ∀ (s : state m) (u' u'' : list (input m)),
+     f s (u' ++ u'') ↔ f (run m s u') u''.
+
+
+Lemma acceptable0 : acc0 (acceptable a).
+Proof. unfold acc0. intro. split; trivial. Qed.
+
+Lemma acceptableT : accT (acceptable a).
+Proof.
+  unfold accT. intros. split; revert s.
+  - induction u' as [| i v IHu].
+    + trivial.
+    + intro. apply IHu.
+  - intro. pose (runC := runC m s u' u'').
+    unfold acceptable. now rewrite <- runC.
+Qed.
+
+Section UniquenessTheorem.
+Variable acceptable' : state m → list (input m) → Prop. 
+Hypotheses (H0 : acc0 acceptable')
+           (HT : accT acceptable').
+
+Theorem acceptable_uniqueness : ∀ (s : state m) (u : list (input m)),
+  acceptable' s u ↔ acceptable a s u.
+Proof.
+  intros. revert s.
+  induction u as [| i u' IHu]; intro; simpl.
+  - apply H0.
+  - assert (H : [i] ++ u' = i :: u'). { trivial. }
+    rewrite <- H.
+    split; intro; elim (HT s [i] u'); intros.
+    + apply (IHu (pass m s i)). rewrite run1 in H2.
+      now apply H2.
+    + apply H3. apply IHu. unfold acceptable in H1. simpl in H1. assumption.
+Qed.
+End UniquenessTheorem.
 End AcceptorTheory.
