Concepts.v
@@ -21,11 +21,13 @@ Module ACCEPTOR.
 Import MACHINE.
 Structure Acceptor {m : Machine} := mkAcceptor
 { acceptant : state m → Prop }.
-Definition accept {m : Machine} (a : Acceptor)
-             (s : state m)
-             (u : list (input m)) : Prop
-:= acceptant a (run m s u).
+Definition acceptable
+             {m : Machine}
+             (a : Acceptor)
+             (s : state m) : list (input m) → Prop
+:= fun u => acceptant a (run m s u).
 End ACCEPTOR.
+
 
 Module TRANSDUCER.
 Import MACHINE.
