MachineTheory.v
@@ -4,9 +4,9 @@ Import ListNotations.
 Import MACHINE.
 
 Section MachineTheory.
-Variables (m : Machine).
+Variable m : Machine.
 
-(* State conservation law *)
+(* Rest law *)
 Definition act0 (f : state m → list (input m) → state m)
 := ∀ s : state m, f s [] = s.
 (* Single impact law *)
@@ -31,15 +31,21 @@ Proof.
   - exact (IHu' (pass m s i)).
 Qed.
 
-Theorem run_uniqueness : ∀ (f : state m → list (input m) → state m),
-  act0 f → act1 f → actC f 
-    → ∀ (s : state m) (u : list (input m)), f s u = run m s u.
+Section UniquenessTheorem.
+Variable run' : state m → list (input m) → state m. 
+Hypotheses (H0 : act0 run')
+           (H1 : act1 run')
+           (HC : actC run').
+
+Theorem run_uniqueness : ∀ (s : state m) (u : list (input m)),
+  run' s u = run m s u.
 Proof.
-  intros * H0 H1 HC *. revert s.
+  intros. revert s.
   induction u as [| i u' IHu]; intro; simpl.
   - apply H0.
   - assert (H : [i] ++ u' = i :: u'). { trivial. }
     rewrite <- H. rewrite (HC s [i] u').
     rewrite <- (H1 s). apply IHu.
 Qed.
+End UniquenessTheorem.
 End MachineTheory.
